Supplementary induction lemmas

vsequent.v
@@ -1,3 +1,5 @@
+Require Import FunInd.
+
 Inductive ctx : Set :=
   | ctx_nil : ctx
   | ctx_cons : (nat * bool) -> ctx -> ctx.
@@ -15,7 +17,7 @@ Inductive prop : Set :=
   | p_or : prop -> prop -> prop
   | p_impl : prop -> prop -> prop.
 
-Fixpoint prop_val (c : ctx) (p : prop) {struct p} : option bool :=
+Function prop_val (c : ctx) (p : prop) {struct p} : option bool :=
   match p with
   | p_sym n => ctx_v n c
   | p_neg p =>
@@ -52,11 +54,18 @@ Fixpoint prop_val (c : ctx) (p : prop) {struct p} : option bool :=
       end
   end.
 
+Lemma prop_val_neg : forall c p b,
+  prop_val c p = Some b -> prop_val c (p_neg p) = Some (negb b).
+Proof.
+  intros c p b H.
+  rewrite prop_val_equation. rewrite -> H. reflexivity.
+Qed.
+
 Inductive s_l : Set :=
   | s_l_nil : s_l
   | s_l_cons : prop -> s_l -> s_l.
 
-Fixpoint s_l_val (c : ctx) (s : s_l) {struct s} : option bool :=
+Function s_l_val (c : ctx) (s : s_l) {struct s} : option bool :=
   match s with
   | s_l_nil => Some true
   | s_l_cons p s =>
@@ -70,24 +79,20 @@ Fixpoint s_l_val (c : ctx) (s : s_l) {struct s} : option bool :=
       end
   end.
 
-Lemma s_l_val_ind : forall c p s b,
-  s_l_val c (s_l_cons p s) = Some b -> (exists b1 b2,
-  (b = andb b1 b2) /\ prop_val c p = Some b1 /\ s_l_val c s = Some b2).
+Lemma s_l_val_lem : forall c p s b0 b1,
+  s_l_val c s = Some b0 -> prop_val c p = Some b1 ->
+  s_l_val c (s_l_cons p s) = Some (andb b1 b0).
 Proof.
-  intros c p s b Heq.
-  induction s.
-    case_eq (prop_val c p).
-      intros b1 Hprop. exists b1. exists true.
-      unfold s_l_val in Heq. rewrite -> Hprop in Heq. inversion Heq. auto.
-      intros Hprop. unfold s_l_val in Heq. rewrite -> Hprop in Heq. discriminate.
-Admitted.
-    
+  intros c p s b0 b1 Hs Hp.
+  rewrite -> (s_l_val_equation c (s_l_cons p s)).
+  rewrite -> Hp. rewrite -> Hs. reflexivity.
+Qed.
 
 Inductive s_r : Set :=
   | s_r_nil : s_r
   | s_r_cons : prop -> s_r -> s_r.
 
-Fixpoint s_r_val (c : ctx) (s : s_r) {struct s} : option bool :=
+Function s_r_val (c : ctx) (s : s_r) {struct s} : option bool :=
   match s with
   | s_r_nil => Some false
   | s_r_cons p s =>
@@ -149,18 +154,17 @@ Inductive eval : seq_t -> seq_t -> Prop :=
       eval (seq l (s_r_cons (p_neg p) r))
            (seq (s_l_cons p l) r).
 
-
 Lemma eval_preserves_val : forall c s1 s2 b,
   eval s1 s2 -> seq_val c s1 = Some b -> seq_val c s2 = Some b.
 Proof.
   intros c s1 s2 b Hev Heq. induction Hev.
     apply (satisfying_ctx_l c (s_l_cons (p_neg p) l) r b) in Heq.
     destruct Heq as [ b1 [ b2 [ Hl [ Hr Himpl ] ] ] ].
+    case_eq (prop_val c p).
+      intros b0 Hprop.
+      apply prop_val_neg in Hprop as Hprop_neg.
+      rewrite s_l_val_equation in Hl.
+      rewrite -> Hprop_neg in Hl.
+      unfold seq_val.
 
-    (* apply (satisfying_ctx_l c (s_l_cons (p_neg p) l) r b1) in Hl. *)
-    (* pose proof (s_l_val_ind c) as Hind. *)
-    (* destruct b; destruct b1; destruct b2. *)
-      (* pose proof (s_l_val_ind c) as Hind. *)
-      (* pose proof (s_l_val_ind c) as Hind.
-    apply (satisfying_ctx_r c l (s_r_cons p r) true true true). *)
 Admitted.
